Imperative/file_input.dfy
@@ -6,6 +6,8 @@ module {:extern "FileInput"} FileInput {
     static function {:extern "shouldEncode"} shouldEncode() : bool
     static function {:extern "getContent"} getContent() : array<byte>
     static method {:extern "putContent"} putContent(x : array<byte>, size : uint32)
-    static function {:extern "getTimestamp"} getTimestamp() : int 
+    static function {:extern "getTimestamp"} getTimestamp() : int
+    static function {:extern "getChannels"} getChannels() : byte
+    ensures 3 <= getChannels() as int <= 4
   }
 }
